theories/FOL/ModelTheory/AnalysisLS.v
@@ -6,15 +6,15 @@ Require Import Undecidability.FOL.ModelTheory.Core.
 Section LSiffDC.
 
     Corollary LS_iff_DC_under_AC00_LEM: 
-        AC00 -> LEM -> LS <-> DC.
+        AC00 -> LEM -> DLS <-> DC.
     Proof.
         intros H1 H2; split.
         - eapply LS_CC_impl_DC; eauto.
-        - intros DC. eapply LS_downward_with_DC_LEM; eauto.
+        - intros DC. eapply LS_correct, LS_downward_with_DC_LEM; eauto.
     Qed.
 
     Corollary LS_iff_DC_BDP_BEP_under_AC00:
-        AC00 -> LS <-> DC /\ BDP /\ BEP.
+        AC00 -> DLS <-> DC /\ BDP /\ BEP.
     Proof.
         intros H1; split.
         - intros HLS. repeat split.
@@ -22,11 +22,11 @@ Section LSiffDC.
           now apply LS_impl_BDP.
           now apply LS_impl_BEP.
         - intros (h1 & h2 & h3).
-          now apply LS_downward_with_BDP_BEP_DC.
+          now apply LS_correct, LS_downward_with_BDP_BEP_DC.
     Qed.
 
     Corollary LS_iff_DDC_BDP_BEP_BCC:
-        LS <-> DDC /\ BDP /\ BEP /\ BCC.
+        DLS <-> DDC /\ BDP /\ BEP /\ BCC.
     Proof.
         split.
         - intros HLS. repeat split.
@@ -34,9 +34,9 @@ Section LSiffDC.
           assert (BDC2) as H2. intros X. now apply OBDC_impl_BDC2_on.
           now apply BDC2_iff_DDC_BCC.
           now apply LS_impl_BDP. now apply LS_impl_BEP.
-          now apply LS_impl_BCC.
+          now eapply BDC_impl_BCC, LS_impl_BDC. 
         - intros (h1 & h2 & h3 & h4).
-          now apply LS_downward.
+          now apply LS_correct, LS_downward.
     Qed.
 
 End LSiffDC.
